Source/DafnyCore/Resolver/PreType/PreTypeResolve.Statements.cs
@@ -18,6 +18,7 @@ namespace Microsoft.Dafny {
 
     public Scope<LabeledStatement> EnclosingStatementLabels { get; set; }
 
+    [CanBeNull] public MethodOrConstructor EnclosingMethodCall { get; set; }
     public Scope<Formal> EnclosingInputParameterFormals { get; set; }
 
     public List<LabeledStatement> LoopStack {
@@ -306,13 +307,16 @@ namespace Microsoft.Dafny {
           // clear the labels for the duration of checking the body, because break statements are not allowed to leave a forall statement
           var prevLblStmts = EnclosingStatementLabels;
           var prevFormals = EnclosingInputParameterFormals;
+          var prevMethodCall = EnclosingMethodCall;
           var prevLoopStack = loopStack;
           EnclosingStatementLabels = new Scope<LabeledStatement>(resolver.Options);
           EnclosingInputParameterFormals = new Scope<Formal>(resolver.Options);
+          EnclosingMethodCall = null;
           loopStack = [];
           ResolveStatement(s.Body, resolutionContext);
           EnclosingStatementLabels = prevLblStmts;
           EnclosingInputParameterFormals = prevFormals;
+          EnclosingMethodCall = prevMethodCall;
           loopStack = prevLoopStack;
         }
         scope.PopMarker();
@@ -505,9 +509,11 @@ namespace Microsoft.Dafny {
         // clear the labels for the duration of checking the hints, because break statements are not allowed to leave a forall statement
         var prevLblStmts = EnclosingStatementLabels;
         var prevFormals = EnclosingInputParameterFormals;
+        var prevMethodCall = EnclosingMethodCall;
         var prevLoopStack = loopStack;
         EnclosingStatementLabels = new Scope<LabeledStatement>(resolver.Options);
         EnclosingInputParameterFormals = new Scope<Formal>(resolver.Options);
+        EnclosingMethodCall = null;
 
         loopStack = [];
         foreach (var h in s.Hints) {
@@ -519,6 +525,7 @@ namespace Microsoft.Dafny {
         }
         EnclosingStatementLabels = prevLblStmts;
         EnclosingInputParameterFormals = prevFormals;
+        EnclosingMethodCall = prevMethodCall;
         loopStack = prevLoopStack;
       }
       if (prevErrorCount == ErrorCount && s.Lines.Count > 0) {
