Source/DafnyCore/Resolver/PreType/PreTypeResolve.cs
@@ -472,6 +472,7 @@ namespace Microsoft.Dafny {
       EnclosingStatementLabels = new Scope<LabeledStatement>(resolver.Options);
       DominatingStatementLabels = new Scope<Label>(resolver.Options);
       EnclosingInputParameterFormals = new Scope<Formal>(resolver.Options);
+      EnclosingMethodCall = null;
       Constraints = new PreTypeConstraints(this);
     }
 
